separate file BuildTree for section 6.3

Pdl/TableauGame.lean
@@ -3,7 +3,7 @@ import Pdl.LocalAll
 import Pdl.Modelgraphs
 import Pdl.StayingInFL
 
-/-! # The Tableau Game (Section 6.2 and 6.3) -/
+/-! # The Tableau Game (Section 6.2) -/
 
 /-! ## Prover and Builder positions -/
 
@@ -12,7 +12,7 @@ notation "Prover" => Player.A
 notation "Builder" => Player.B
 
 inductive ProverPos (H : History) (X : Sequent) : Type where
-  | nlpRep : ¬ Nonempty (LoadedPathRepeat H X) → ProverPos H X -- Prover loses
+  | nlpRep : rep H X → ¬ Nonempty (LoadedPathRepeat H X) → ProverPos H X -- Prover loses
   | bas : ¬ rep H X → X.basic → ProverPos H X -- Prover must apply a PDL rule
   | nbas : ¬ rep H X → ¬ X.basic → ProverPos H X -- Prover must make a local LocalTableau
   deriving DecidableEq
@@ -31,7 +31,7 @@ def posOf (H : History) (X : Sequent) : ProverPos H X ⊕ BuilderPos H X :=
   then .inr (.lpr (.choice neNlp)) -- BuilderPos with no moves to let Prover win at lpr
   else
     if rep : rep H X
-    then .inl (.nlpRep neNlp) -- ProverPos with no moves to let Builder win at (non-lp) repeat
+    then .inl (.nlpRep rep neNlp) -- ProverPos with no moves to let Builder win at (non-lp) repeat
     else
       if bas : X.basic
       then .inl (.bas rep bas) -- actual ProverPos to choose a PDL rule
@@ -66,7 +66,7 @@ With `move_of_mem_theMoves` and `mem_theMoves_of_move` this agrees with `move`. 
 @[simp]
 def theMoves : GamePos → Finset GamePos
   -- ProverPos:
-  | ⟨H, X, .inl (.nlpRep _)⟩ => ∅ -- no moves ⇒ Builder wins
+  | ⟨H, X, .inl (.nlpRep _ _)⟩ => ∅ -- no moves ⇒ Builder wins
   | ⟨H, X, .inl (.bas _ Xbasic)⟩ =>
       -- need to choose PDL rule application:
       match X with
@@ -1131,7 +1131,7 @@ lemma tableauGame_turn_Builder {Hist X lpr} :
 
 @[simp]
 lemma tableauGame_winner_nlpRep_eq_Builder :
-    @winner i tableauGame sI sJ ⟨Hist, X, .inl (.nlpRep h1)⟩ = Builder := by
+    @winner i tableauGame sI sJ ⟨Hist, X, .inl (.nlpRep h1 h2)⟩ = Builder := by
   simp [winner, tableauGame]
 
 @[simp]
@@ -1339,236 +1339,3 @@ def startPos (X : Sequent) : GamePos := ⟨[], X, posOf [] X⟩
 /-- If Prover has a winning strategy then there is a closed tableau. -/
 theorem gameP (X : Sequent) (s : Strategy tableauGame Prover) (h : winning s (startPos X)) :
     Nonempty (Tableau [] X) := gameP_general [] X s _ h
-
-/-! ## All applicable PDL rules
-
-FIXME move this section to another file? It is like `LocalAll.lean` but not local.
--/
-
-/-- List of all `PdlRule`s applicable to `X`. Code is based on part of `theMoves`. -/
-def PdlRule.all (X : Sequent) : List (Σ Y, PdlRule X Y) :=
-  match X with
-  | ⟨L, R, none⟩ => -- (L+) if X is not loaded, choice of formula
-        (L.attach.map (fun -- Catch a negation and all boxes (≥ 1) after it to be loaded.
-                    | ⟨~φ, in_L⟩ => match bdef : boxesOf φ with
-                        | (δ@δ_def:(_::_), ψ) =>
-                          have notBox : ¬ ψ.isBox := by
-                            have := @boxesOf_output_not_isBox φ; simp_all
-                          have _in'' : (~⌈⌈δ.dropLast⌉⌉⌈δ.getLast _⌉ψ) ∈ L := by
-                            rw [def_of_boxesOf_def bdef] at in_L
-                            convert in_L using 2
-                            rw [← δ_def, ← @boxes_last, @List.dropLast_append_getLast]
-                          [ ⟨ ( L.erase _, R
-                              , some (Sum.inl (~'(⌊⌊δ.dropLast⌋⌋⌊δ.getLast (by simp_all)⌋ψ))))
-                            , .loadL _in'' notBox rfl ⟩ ]
-                        | ([],_) => []
-                    | _ => [] )).flatten
-        ++
-        (R.attach.map (fun
-                    | ⟨~φ, in_R⟩ => match bdef : boxesOf φ with
-                        | (δ@δ_def:(_::_), ψ) =>
-                          have notBox : ¬ ψ.isBox := by
-                            have := @boxesOf_output_not_isBox φ; simp_all
-                          have _in'' : (~⌈⌈δ.dropLast⌉⌉⌈δ.getLast _⌉ψ) ∈ R := by
-                            rw [def_of_boxesOf_def bdef] at in_R
-                            convert in_R using 2
-                            rw [← δ_def, ← @boxes_last, @List.dropLast_append_getLast]
-                          [ ⟨ ( L, R.erase _
-                              , some (Sum.inr (~'(⌊⌊δ.dropLast⌋⌋⌊δ.getLast (by simp_all)⌋ψ))))
-                            , .loadR _in'' notBox rfl ⟩ ]
-                        | ([],_) => []
-                    | _ => [] )).flatten
-  | ⟨L, R, some (.inl (~'⌊·a⌋ξ))⟩ =>
-          ( match ξ_def : ξ with -- (M) rule, deterministic:
-          | .normal φ => [ ⟨ ⟨ _, _, none                ⟩, .modL rfl rfl ⟩ ]
-          | .loaded χ => [ ⟨ ⟨ _, _, some (Sum.inl (~'χ))⟩, .modL rfl rfl ⟩ ] )
-          ++ -- (L-) rule, deterministic:
-          [ match ξsp_def : ξ.split with
-          | ⟨δs, φ⟩ => match sp_def : splitLast δs with
-            | none =>
-              ⟨ (L.insert (~(⌊·a⌋ξ).unload), R, none)
-              , @PdlRule.freeL _ L R [] (·a) φ _
-                  (by simp_all [nil_of_splitLast_none, AnyFormula.split_eq_nil_is_normal])
-                  (by simp_all [nil_of_splitLast_none, AnyFormula.split_eq_nil_is_normal]) ⟩
-            | some ⟨δs_, δ⟩ =>
-              ⟨ (L.insert (~(⌊·a⌋ξ).unload), R, none)
-              , by
-                  have ξ_def : ξ = AnyFormula.loadBoxes (δs_ ++ [δ]) φ := by
-                      rw [← splitLast_append_singleton] at sp_def
-                      rw [splitLast_inj sp_def, ← loadMulti_split] at ξsp_def
-                      have : (loadMulti δs_ δ φ).split = AnyFormula.split (loadMulti δs_ δ φ) := rfl
-                      have := AnyFormula.split_inj (this ▸ ξsp_def)
-                      exact this ▸ loadMulti_eq_loadBoxes
-                  refine @PdlRule.freeL _ L R (·a :: δs_) δ φ _ ?_ ?_
-                  · simp [ξ_def, box_loadBoxes_append_eq_of_loaded_eq_loadBoxes]
-                  · simp only [Formula.boxes_cons, Prod.mk.injEq, and_true]
-                    convert rfl
-                    simp [ξ_def, AnyFormula.loadBoxes_unload_eq_boxes, boxes_last] ⟩
-          ]
-  | ⟨L, R, some (.inr (~'⌊·a⌋ξ))⟩ =>
-          ( match ξ_def : ξ with -- (M) rule, deterministic:
-          | .normal φ => [ ⟨ ⟨ _, _, none                ⟩, .modR rfl rfl ⟩ ]
-          | .loaded χ => [ ⟨ ⟨ _, _, some (Sum.inr (~'χ))⟩, .modR rfl rfl ⟩ ] )
-          ++ -- (L-) rule, deterministic:
-          [ match ξsp_def : ξ.split with
-          | ⟨δs, φ⟩ => match sp_def : splitLast δs with
-            | none =>
-              ⟨ (L, R.insert (~(⌊·a⌋ξ).unload), none)
-              , @PdlRule.freeR _ L R [] (·a) φ _
-                  (by simp_all [nil_of_splitLast_none, AnyFormula.split_eq_nil_is_normal])
-                  (by simp_all [nil_of_splitLast_none, AnyFormula.split_eq_nil_is_normal]) ⟩
-            | some ⟨δs_, δ⟩ =>
-              ⟨ (L, R.insert (~(⌊·a⌋ξ).unload), none)
-              , by
-                  have ξ_def : ξ = AnyFormula.loadBoxes (δs_ ++ [δ]) φ := by
-                      rw [← splitLast_append_singleton] at sp_def
-                      rw [splitLast_inj sp_def, ← loadMulti_split] at ξsp_def
-                      have : (loadMulti δs_ δ φ).split = AnyFormula.split (loadMulti δs_ δ φ) := rfl
-                      have := AnyFormula.split_inj (this ▸ ξsp_def)
-                      exact this ▸ loadMulti_eq_loadBoxes
-                  refine @PdlRule.freeR _ L R (·a :: δs_) δ φ _ ?_ ?_
-                  · simp [ξ_def, box_loadBoxes_append_eq_of_loaded_eq_loadBoxes]
-                  · simp only [Formula.boxes_cons, Prod.mk.injEq, and_true, true_and]
-                    convert rfl
-                    simp [ξ_def, AnyFormula.loadBoxes_unload_eq_boxes, boxes_last] ⟩
-          ]
-  -- WORRY: also need to allow freeL/freeR from non-atomic loading? (to make _spec below provable)
-  | _ => [] -- YOLO?
-
-/-- NOTE: unfinished but also NOT USED at the moment / not needed at all?
-
-Maybe it's enough to build the countermodelgraph from a buildTree that uses only the PdlRules in
-`PdlRule.all` and we can ignore other (e.g. non-atomic unloading) PdlRule applications???
--/
-lemma PdlRule.all_spec {X Y} (r : PdlRule X Y) : ⟨Y, r⟩ ∈ PdlRule.all X := by
-  cases r
-  case loadL L δs α φ R in_L notBox Y_def =>
-    subst Y_def
-    unfold all
-    simp
-    sorry
-  case loadR R δs α φ L in_R notBox Y_def =>
-    -- analogous
-    sorry
-  case freeL L R δs α φ X_def Y_def =>
-    subst X_def Y_def
-    cases δs <;> simp_all [all]
-    · -- rw [Formula.boxes_nil] -- motive is not type correct
-      sorry
-    · sorry
-  case freeR L R δs α φ X_def Y_def =>
-    -- analogous
-    sorry
-  case modL L R a ξ X_def Y_def =>
-    subst X_def Y_def
-    cases ξ <;> simp_all [all]
-  case modR L R a ξ X_def Y_def =>
-    subst X_def Y_def
-    cases ξ <;> simp_all [all]
-
-/-! ## From Builder winning strategies to model graphs (Section 6.3) -/
-
--- See also Bml/CompletenessViaPaths.lean for inspiration that might be useful here.
-
-/-- Tree data type to keep track of choices made by Builder. Might still need to be tweaked.
-- Choices should be labelled with the choices made by prover?
-- Maybe we also need to carry proofs in here?
--/
-inductive BuildTree : Sequent → Type
-  | Leaf {X} : BuildTree X
-  | Step {X} : List (Σ Y, BuildTree Y) → BuildTree X
-
-/-- The tree generated from a winning Builder strategy -/
-def buildTree (s : Strategy tableauGame Builder) {H X} p (h : winning s ⟨H, X, p⟩) : BuildTree X :=
-  match p with
-  -- Prover positions:
-  | Sum.inl (.nlpRep _) => .Leaf -- Builder wins :-)
-  | Sum.inl (.bas nrep bas) => -- prover chooses PDL rule
-      let prMoves := (PdlRule.all X).map
-        (fun ⟨Y, r⟩ => (⟨(X :: H), Y, posOf (X :: H) Y⟩ : GamePos))
-      have stillWin : ∀ newPos ∈ prMoves, winning s newPos := by
-        -- FIXME some redundancy between here and the termination proof
-        intro newPos newPos_in
-        refine @winning_of_whatever_other_move _ _ s _ (by simp) h ⟨newPos, ?_⟩
-        simp only [List.mem_map, Sigma.exists, exists_and_right, prMoves] at newPos_in
-        rcases newPos_in with ⟨Y, ⟨r, r_in⟩, def_newPos⟩
-        simp only [tableauGame]
-        apply mem_theMoves_of_move
-        subst newPos
-        refine move.prPdl r
-      .Step <| prMoves.attach.map <| fun ⟨pos, h⟩ => ⟨pos.2.1, buildTree s pos.2.2 (stillWin pos h)⟩
-  | Sum.inl (.nbas nrep nbas) => -- prover chooses a local tableau
-      -- Note: not using the Fintype instance because we want a List, not Finset
-      let prMoves := (LocalTableau.all X).map
-        (fun ltab => (⟨H, X, .inr (.ltab nrep nbas ltab)⟩ : GamePos))
-      have stillWin : ∀ newPos ∈ prMoves, winning s newPos := by
-        intro newPos newPos_in
-        refine @winning_of_whatever_other_move _ _ s _ (by simp) h ⟨newPos, ?_⟩
-        simp only [tableauGame, List.mem_map, theMoves, Finset.mem_image, prMoves] at *
-        rcases newPos_in with ⟨ltX, ltX_in, def_newPos⟩
-        refine ⟨ltX, ?_, def_newPos⟩
-        simp_all [Fintype.elems]
-      .Step <| prMoves.attach.map <| fun ⟨pos, h⟩ => ⟨pos.2.1, buildTree s pos.2.2 (stillWin pos h)⟩
-  -- Builder positions:
-  | Sum.inr (.lpr _) => by exfalso; simp [winning] at h -- prover wins, cannot happen
-  | Sum.inr (.ltab nrep nbas ltX) =>
-      if ne : (tableauGame.moves ⟨H, ⟨X, Sum.inr (BuilderPos.ltab nrep nbas ltX)⟩⟩).Nonempty
-      then
-        -- use `s` to choose `Y ∈ endNodeOf ltX`
-        let Y := (s ⟨H, X, Sum.inr (.ltab nrep nbas ltX)⟩ (by simp) ne)
-        have new_h : winning s Y.1 := winning_of_winning_move _ h
-        have forTermination : move ⟨H, X, Sum.inr (.ltab nrep nbas ltX)⟩ Y.1 := by
-          have := Y.2
-          simp only [Game.Pos.moves, tableauGame, theMoves, List.mem_toFinset] at this
-          have := fun Y => @move.buEnd X ltX Y H nrep nbas
-          grind
-        .Step [ ⟨_, buildTree s _ new_h⟩ ]
-      else by
-        exfalso
-        simp_all [winning, winner]
-termination_by
-  tableauGame.wf.2.wrap (⟨H, X, p⟩ : GamePos)
-decreasing_by
-  · simp_wf
-    simp only [tableauGame, Game.wf, WellFoundedRelation.rel]
-    -- PDL rule case
-    simp only [List.mem_map, Sigma.exists, exists_and_right, prMoves] at h
-    rcases h with ⟨Y, ⟨r, _⟩, def_newPos⟩
-    subst def_newPos
-    exact move.prPdl r
-  · simp_wf
-    simp only [tableauGame, Game.wf, WellFoundedRelation.rel]
-    -- show that it's a move
-    unfold prMoves at h
-    simp only [List.mem_map] at h
-    rcases h with ⟨ltX, _, def_pos⟩
-    subst def_pos
-    apply @move.prLocTab H X nrep nbas
-  · simp_wf
-    simp only [tableauGame, Game.wf, WellFoundedRelation.rel]
-    -- show that it's a move
-    exact forTermination
-
--- IDEA: define paths inside BuildTree like in `TableauPath.lean`?
--- Then define *maximal* paths? Including going via back-edges!?
-
--- TODO Definition 6.13 initial, pre-state
-
--- TODO Lemma 6.14: how to collect formulas in a pre-state
-
--- TODO Lemma 6.15
-
--- TODO Lemma 6.16 pre-states are locally consistent and saturated, last node basic.
-
--- TODO Definition 6.18 to get model graph from strategy tree.
-
--- TODO Lemma 6.18
-
--- TODO Lemma 6.19: for any diamond we can go to a pre-state where that diamond is loaded
-
--- TODO Lemma 6.20: diamond existence lemma for pre-states
-
-/-- Theorem 6.21: If Builder has a winning strategy then there is a model graph. -/
-theorem strmg (X : Sequent) (s : Strategy tableauGame Builder) (h : winning s (startPos X)) :
-    ∃ (WS : Finset (Finset Formula)) (mg : ModelGraph WS), X.toFinset ∈ WS := by
-  sorry
