Pdl/BuildTree.lean
@@ -1,0 +1,243 @@
+import Pdl.TableauGame
+
+/-! # From winning strategies to model graphs (Section 6.3) -/
+
+/-- List of all `PdlRule`s applicable to `X`. Code is based on part of `theMoves`
+This is also similar to the definitions in `LocalAll.lean`. -/
+def PdlRule.all (X : Sequent) : List (Σ Y, PdlRule X Y) :=
+  match X with
+  | ⟨L, R, none⟩ => -- (L+) if X is not loaded, choice of formula
+        (L.attach.map (fun -- Catch a negation and all boxes (≥ 1) after it to be loaded.
+                    | ⟨~φ, in_L⟩ => match bdef : boxesOf φ with
+                        | (δ@δ_def:(_::_), ψ) =>
+                          have notBox : ¬ ψ.isBox := by
+                            have := @boxesOf_output_not_isBox φ; simp_all
+                          have _in'' : (~⌈⌈δ.dropLast⌉⌉⌈δ.getLast _⌉ψ) ∈ L := by
+                            rw [def_of_boxesOf_def bdef] at in_L
+                            convert in_L using 2
+                            rw [← δ_def, ← @boxes_last, @List.dropLast_append_getLast]
+                          [ ⟨ ( L.erase _, R
+                              , some (Sum.inl (~'(⌊⌊δ.dropLast⌋⌋⌊δ.getLast (by simp_all)⌋ψ))))
+                            , .loadL _in'' notBox rfl ⟩ ]
+                        | ([],_) => []
+                    | _ => [] )).flatten
+        ++
+        (R.attach.map (fun
+                    | ⟨~φ, in_R⟩ => match bdef : boxesOf φ with
+                        | (δ@δ_def:(_::_), ψ) =>
+                          have notBox : ¬ ψ.isBox := by
+                            have := @boxesOf_output_not_isBox φ; simp_all
+                          have _in'' : (~⌈⌈δ.dropLast⌉⌉⌈δ.getLast _⌉ψ) ∈ R := by
+                            rw [def_of_boxesOf_def bdef] at in_R
+                            convert in_R using 2
+                            rw [← δ_def, ← @boxes_last, @List.dropLast_append_getLast]
+                          [ ⟨ ( L, R.erase _
+                              , some (Sum.inr (~'(⌊⌊δ.dropLast⌋⌋⌊δ.getLast (by simp_all)⌋ψ))))
+                            , .loadR _in'' notBox rfl ⟩ ]
+                        | ([],_) => []
+                    | _ => [] )).flatten
+  | ⟨L, R, some (.inl (~'⌊·a⌋ξ))⟩ =>
+          ( match ξ_def : ξ with -- (M) rule, deterministic:
+          | .normal φ => [ ⟨ ⟨ _, _, none                ⟩, .modL rfl rfl ⟩ ]
+          | .loaded χ => [ ⟨ ⟨ _, _, some (Sum.inl (~'χ))⟩, .modL rfl rfl ⟩ ] )
+          ++ -- (L-) rule, deterministic:
+          [ match ξsp_def : ξ.split with
+          | ⟨δs, φ⟩ => match sp_def : splitLast δs with
+            | none =>
+              ⟨ (L.insert (~(⌊·a⌋ξ).unload), R, none)
+              , @PdlRule.freeL _ L R [] (·a) φ _
+                  (by simp_all [nil_of_splitLast_none, AnyFormula.split_eq_nil_is_normal])
+                  (by simp_all [nil_of_splitLast_none, AnyFormula.split_eq_nil_is_normal]) ⟩
+            | some ⟨δs_, δ⟩ =>
+              ⟨ (L.insert (~(⌊·a⌋ξ).unload), R, none)
+              , by
+                  have ξ_def : ξ = AnyFormula.loadBoxes (δs_ ++ [δ]) φ := by
+                      rw [← splitLast_append_singleton] at sp_def
+                      rw [splitLast_inj sp_def, ← loadMulti_split] at ξsp_def
+                      have : (loadMulti δs_ δ φ).split = AnyFormula.split (loadMulti δs_ δ φ) := rfl
+                      have := AnyFormula.split_inj (this ▸ ξsp_def)
+                      exact this ▸ loadMulti_eq_loadBoxes
+                  refine @PdlRule.freeL _ L R (·a :: δs_) δ φ _ ?_ ?_
+                  · simp [ξ_def, box_loadBoxes_append_eq_of_loaded_eq_loadBoxes]
+                  · simp only [Formula.boxes_cons, Prod.mk.injEq, and_true]
+                    convert rfl
+                    simp [ξ_def, AnyFormula.loadBoxes_unload_eq_boxes, boxes_last] ⟩
+          ]
+  | ⟨L, R, some (.inr (~'⌊·a⌋ξ))⟩ =>
+          ( match ξ_def : ξ with -- (M) rule, deterministic:
+          | .normal φ => [ ⟨ ⟨ _, _, none                ⟩, .modR rfl rfl ⟩ ]
+          | .loaded χ => [ ⟨ ⟨ _, _, some (Sum.inr (~'χ))⟩, .modR rfl rfl ⟩ ] )
+          ++ -- (L-) rule, deterministic:
+          [ match ξsp_def : ξ.split with
+          | ⟨δs, φ⟩ => match sp_def : splitLast δs with
+            | none =>
+              ⟨ (L, R.insert (~(⌊·a⌋ξ).unload), none)
+              , @PdlRule.freeR _ L R [] (·a) φ _
+                  (by simp_all [nil_of_splitLast_none, AnyFormula.split_eq_nil_is_normal])
+                  (by simp_all [nil_of_splitLast_none, AnyFormula.split_eq_nil_is_normal]) ⟩
+            | some ⟨δs_, δ⟩ =>
+              ⟨ (L, R.insert (~(⌊·a⌋ξ).unload), none)
+              , by
+                  have ξ_def : ξ = AnyFormula.loadBoxes (δs_ ++ [δ]) φ := by
+                      rw [← splitLast_append_singleton] at sp_def
+                      rw [splitLast_inj sp_def, ← loadMulti_split] at ξsp_def
+                      have : (loadMulti δs_ δ φ).split = AnyFormula.split (loadMulti δs_ δ φ) := rfl
+                      have := AnyFormula.split_inj (this ▸ ξsp_def)
+                      exact this ▸ loadMulti_eq_loadBoxes
+                  refine @PdlRule.freeR _ L R (·a :: δs_) δ φ _ ?_ ?_
+                  · simp [ξ_def, box_loadBoxes_append_eq_of_loaded_eq_loadBoxes]
+                  · simp only [Formula.boxes_cons, Prod.mk.injEq, and_true, true_and]
+                    convert rfl
+                    simp [ξ_def, AnyFormula.loadBoxes_unload_eq_boxes, boxes_last] ⟩
+          ]
+  -- WORRY: also need to allow freeL/freeR from non-atomic loading? (to make _spec below provable)
+  | _ => [] -- YOLO?
+
+/-- NOTE: unfinished but also NOT USED at the moment / not needed at all?
+
+Maybe it's enough to build the countermodelgraph from a buildTree that uses only the PdlRules in
+`PdlRule.all` and we can ignore other (e.g. non-atomic unloading) PdlRule applications???
+-/
+lemma PdlRule.all_spec {X Y} (r : PdlRule X Y) : ⟨Y, r⟩ ∈ PdlRule.all X := by
+  cases r
+  case loadL L δs α φ R in_L notBox Y_def =>
+    subst Y_def
+    unfold all
+    simp
+    sorry
+  case loadR R δs α φ L in_R notBox Y_def =>
+    -- analogous
+    sorry
+  case freeL L R δs α φ X_def Y_def =>
+    subst X_def Y_def
+    cases δs <;> simp_all [all]
+    · -- rw [Formula.boxes_nil] -- motive is not type correct
+      sorry
+    · sorry
+  case freeR L R δs α φ X_def Y_def =>
+    -- analogous
+    sorry
+  case modL L R a ξ X_def Y_def =>
+    subst X_def Y_def
+    cases ξ <;> simp_all [all]
+  case modR L R a ξ X_def Y_def =>
+    subst X_def Y_def
+    cases ξ <;> simp_all [all]
+
+
+-- See also Bml/CompletenessViaPaths.lean for inspiration that might be useful here.
+
+/-- Tree data type to keep track of choices made by Builder. Might still need to be tweaked.
+- Choices should be labelled with the choices made by prover?
+- Maybe we also need to carry proofs in here?
+-/
+inductive BuildTree : Sequent → Type
+  | Leaf {X} : Nat → BuildTree X
+  | Step {X} : List (Σ Y, BuildTree Y) → BuildTree X
+
+-- QUESTION: are actually all leafs in the BuildTree backpointers?
+
+def theRep {H X} (rp : rep H X) : Nat :=
+  match h : List.findIdx? (fun Y => decide (Y.setEqTo X)) H with
+  | none => by
+      exfalso
+      have : ∃ Y ∈ H, decide (Y.setEqTo X) = true := by aesop
+      have := @List.findIdx?_eq_some_of_exists Sequent H (fun Y => Y.setEqTo X) this
+      simp_all
+  | some k => k
+
+/-- The tree generated from a winning Builder strategy -/
+def buildTree (s : Strategy tableauGame Builder) {H X} p (h : winning s ⟨H, X, p⟩) : BuildTree X :=
+  match p with
+  -- Prover positions:
+  | Sum.inl (.nlpRep rp noLpRep) => .Leaf (theRep rp) -- Builder wins with back-pointer :-)
+  | Sum.inl (.bas nrep bas) => -- prover chooses PDL rule
+      let prMoves := (PdlRule.all X).map
+        (fun ⟨Y, r⟩ => (⟨(X :: H), Y, posOf (X :: H) Y⟩ : GamePos))
+      have stillWin : ∀ newPos ∈ prMoves, winning s newPos := by
+        -- FIXME some redundancy between here and the termination proof
+        intro newPos newPos_in
+        refine @winning_of_whatever_other_move _ _ s _ (by simp) h ⟨newPos, ?_⟩
+        simp only [List.mem_map, Sigma.exists, exists_and_right, prMoves] at newPos_in
+        rcases newPos_in with ⟨Y, ⟨r, r_in⟩, def_newPos⟩
+        simp only [tableauGame]
+        apply mem_theMoves_of_move
+        subst newPos
+        refine move.prPdl r
+      .Step <| prMoves.attach.map <| fun ⟨pos, h⟩ => ⟨pos.2.1, buildTree s pos.2.2 (stillWin pos h)⟩
+  | Sum.inl (.nbas nrep nbas) => -- prover chooses a local tableau
+      -- Note: not using the Fintype instance because we want a List, not Finset
+      let prMoves := (LocalTableau.all X).map
+        (fun ltab => (⟨H, X, .inr (.ltab nrep nbas ltab)⟩ : GamePos))
+      have stillWin : ∀ newPos ∈ prMoves, winning s newPos := by
+        intro newPos newPos_in
+        refine @winning_of_whatever_other_move _ _ s _ (by simp) h ⟨newPos, ?_⟩
+        simp only [tableauGame, List.mem_map, theMoves, Finset.mem_image, prMoves] at *
+        rcases newPos_in with ⟨ltX, ltX_in, def_newPos⟩
+        refine ⟨ltX, ?_, def_newPos⟩
+        simp_all [Fintype.elems]
+      .Step <| prMoves.attach.map <| fun ⟨pos, h⟩ => ⟨pos.2.1, buildTree s pos.2.2 (stillWin pos h)⟩
+  -- Builder positions:
+  | Sum.inr (.lpr _) => by exfalso; simp [winning] at h -- prover wins, cannot happen
+  | Sum.inr (.ltab nrep nbas ltX) =>
+      if ne : (tableauGame.moves ⟨H, ⟨X, Sum.inr (BuilderPos.ltab nrep nbas ltX)⟩⟩).Nonempty
+      then
+        -- use `s` to choose `Y ∈ endNodeOf ltX`
+        let Y := (s ⟨H, X, Sum.inr (.ltab nrep nbas ltX)⟩ (by simp) ne)
+        have new_h : winning s Y.1 := winning_of_winning_move _ h
+        have forTermination : move ⟨H, X, Sum.inr (.ltab nrep nbas ltX)⟩ Y.1 := by
+          have := Y.2
+          simp only [Game.Pos.moves, tableauGame, theMoves, List.mem_toFinset] at this
+          have := fun Y => @move.buEnd X ltX Y H nrep nbas
+          grind
+        .Step [ ⟨_, buildTree s _ new_h⟩ ]
+      else by
+        exfalso
+        simp_all [winning, winner]
+termination_by
+  tableauGame.wf.2.wrap (⟨H, X, p⟩ : GamePos)
+decreasing_by
+  · simp_wf
+    simp only [tableauGame, Game.wf, WellFoundedRelation.rel]
+    -- PDL rule case
+    simp only [List.mem_map, Sigma.exists, exists_and_right, prMoves] at h
+    rcases h with ⟨Y, ⟨r, _⟩, def_newPos⟩
+    subst def_newPos
+    exact move.prPdl r
+  · simp_wf
+    simp only [tableauGame, Game.wf, WellFoundedRelation.rel]
+    -- show that it's a move
+    unfold prMoves at h
+    simp only [List.mem_map] at h
+    rcases h with ⟨ltX, _, def_pos⟩
+    subst def_pos
+    apply @move.prLocTab H X nrep nbas
+  · simp_wf
+    simp only [tableauGame, Game.wf, WellFoundedRelation.rel]
+    -- show that it's a move
+    exact forTermination
+
+-- IDEA: define paths and edge-relation inside BuildTree as in `TableauPath.lean`?
+-- Then define *maximal* paths? Including going via back-edges!?
+
+-- TODO Definition 6.13 initial, pre-state
+
+-- TODO Lemma 6.14: how to collect formulas in a pre-state
+
+-- TODO Lemma 6.15
+
+-- TODO Lemma 6.16 pre-states are locally consistent and saturated, last node basic.
+
+-- TODO Definition 6.18 to get model graph from strategy tree.
+
+-- TODO Lemma 6.18
+
+-- TODO Lemma 6.19: for any diamond we can go to a pre-state where that diamond is loaded
+
+-- TODO Lemma 6.20: diamond existence lemma for pre-states
+
+/-- Theorem 6.21: If Builder has a winning strategy then there is a model graph. -/
+theorem strmg (X : Sequent) (s : Strategy tableauGame Builder) (h : winning s (startPos X)) :
+    ∃ (WS : Finset (Finset Formula)) (mg : ModelGraph WS), X.toFinset ∈ WS := by
+  let bt := buildTree s (startPos X).2.2
+  sorry
